Insertion between lines in text editor, attempted and failed to use C libraries in GForth

forth_stuff/c_inter.fs
@@ -1,0 +1,4 @@
+( ~/.gforth/ )
+\c #include "basic.h"
+c-function adder add n n -- n
+
