coq_stuff/tutorial.v
@@ -1,36 +1,36 @@
 Set Implicit Arguments.
 Set Asymmetric Patterns.
-Require List.
+Require Import List.
 Open Scope list_scope.
 
 Inductive binop : Set :=
-  Plus | Times.
+  Plus | Times | First | Second.
 
 Inductive exp : Set :=
   | Const : nat -> exp
-  | Binop : binop -> exp -> exp -> exp 
-  | First : exp -> exp -> exp
-  | Second : exp -> exp -> exp.
+  | Binop : binop -> exp -> exp -> exp.
 (* take a binary operation and 2 expressions and return one expression *)
+Fixpoint frs (e1 : nat) (e2 : nat) : nat := e1.
+Fixpoint snd (e1 : nat) (e2 : nat) : nat := e2.
 
 Definition binopDenote := fun b =>
   match b with
   | Plus => plus
   | Times => mult
+  | First => frs
+  | Second => snd
   end.
 
 Fixpoint expDenote ( e : exp) : nat :=
   match e with
   | Const n => n
   | Binop b e1 e2 => (binopDenote b) (expDenote e1) (expDenote e2)
-  | First e1 e2 => expDenote(e1)
-  | Second e1 e2 => expDenote(e2)
   end.
 
 Eval simpl in expDenote (Const 42).
 Eval simpl in expDenote (Binop Plus (Const 2) (Const 3)).
-Eval simpl in expDenote (First (Binop Plus (Const 2) (Const 3)) (Binop Times (Const 2) (Const 3))).
-Eval simpl in expDenote (Second (Binop Plus (Const 2) (Const 3)) (Binop Times (Const 2) (Const 3))).
+Eval simpl in expDenote (Binop First (Binop Plus (Const 2) (Const 3)) (Binop Times (Const 2) (Const 3))).
+Eval simpl in expDenote (Binop Second (Binop Plus (Const 2) (Const 3)) (Binop Times (Const 2) (Const 3))).
 
 Inductive instr : Set :=
   | iConst : nat -> instr
@@ -43,7 +43,41 @@ Definition instrDenote (i : instr) (s: stack) : option stack :=
   | iConst n => Some (n :: s)
   | iBinop b =>
       match s with
-      | (arg1 :: arg2 :: s') => Some ((binopDenote b1) arg1 arg2 :: s')
+      | (arg1 :: arg2 :: s') => Some ((binopDenote b) arg1 arg2 :: s')
       | _ => None
       end
   end.
+
+Fixpoint progDenote (p : prog) (s : stack) : option stack :=
+  match p with
+  | nil => Some s
+  | i :: p' =>
+      match instrDenote i s with
+      | None => None
+      | Some s' => progDenote p' s'
+      end
+  end.
+(* kinda cool how all binary instructions just generalize in the stack machine [they did not but now they do!] *)
+
+Fixpoint compile (e : exp) : prog :=
+  match e with
+  | Const n => iConst n :: nil
+  | Binop b e1 e2 => compile e2 ++ compile e1 ++ iBinop b :: nil
+  end.
+
+Eval simpl in compile (Const 42).
+Eval simpl in progDenote (compile (Binop Times (Binop Second(Const 2) (Const 3)) (Const 7))).
+(* yay! *)
+
+Lemma compile_correct' : forall e p s, progDenote (compile e ++ p) s = progDenote p (expDenote e :: s).
+induction e. intros. unfold compile. unfold expDenote. unfold progDenote at 1. simpl. fold progDenote. reflexivity.
+intros. unfold compile. fold compile. unfold expDenote. fold expDenote. rewrite app_assoc_reverse. rewrite IHe2.
+rewrite app_assoc_reverse. rewrite IHe1. unfold progDenote at 1. simpl. fold progDenote. reflexivity.
+Qed.
+Lemma nr : forall e, compile e = compile e ++ nil.
+intros. rewrite app_nil_r. reflexivity.
+Qed.
+Theorem compile_correct : forall e, progDenote (compile e) nil = Some (expDenote e :: nil).
+intros. rewrite nr. rewrite compile_correct'. reflexivity.
+Qed.
+
